Simplify wfo

nola/util/wfo.v
@@ -6,69 +6,33 @@ From stdpp Require Export well_founded.
 (** ** [wfo]: Type with a well-founded order *)
 
 Structure wfo := Wfo {
+  (** Underlying type *)
   wfo_car :> Type;
   (** Strict order *)
   wfo_lt : wfo_car → wfo_car → Prop;
-  (** Reflexive order *)
-  wfo_le : wfo_car → wfo_car → Prop;
-  (** [wfo_le] is the reflexive closure of [wfo_lt] *)
-  wfo_le_lteq : ∀a b , wfo_le a b ↔ wfo_lt a b ∨ a = b;
-  (** [wfo_lt] is transitive *)
-  wfo_lt_trans : ∀a b c , wfo_lt a b → wfo_lt b c → wfo_lt a c;
   (** [wfo_lt] is well-founded *)
   wfo_lt_wf : wf wfo_lt;
 }.
 
 Arguments wfo_car : simpl never.
 Arguments wfo_lt {A} _ _ : simpl never, rename.
-Arguments wfo_le {A} _ _ : simpl never, rename.
-Arguments wfo_le_lteq {A _ _} : simpl never, rename.
-Arguments wfo_lt_trans {A _ _ _} _ _ : simpl never, rename.
 Arguments wfo_lt_wf {A} : simpl never, rename.
 Infix "≺" := wfo_lt (at level 70, no associativity) : nola_scope.
-Infix "≼" := wfo_le (at level 70, no associativity) : nola_scope.
 
 (** Inverse of [≺] *)
 Definition wfo_gt {A : wfo} (a b : A) := b ≺ a.
 Infix "≻" := wfo_gt (at level 70, no associativity) : nola_scope.
 
-(** Inverse of [≼] *)
-Definition wfo_ge {A : wfo} (a b : A) := b ≼ a.
-Infix "≽" := wfo_ge (at level 70, no associativity) : nola_scope.
-
-(** ** Facts about [wfo] *)
-Section wfo_facts.
-  Context {A : wfo}.
-  Implicit Type a b c : A.
-
-  (** [≼] is reflexive *)
-  Lemma wfo_le_refl a : a ≼ a.
-  Proof. apply wfo_le_lteq. by right. Qed.
-
-  (** Turn [≺] into [≼] *)
-  Lemma wfo_lt_le a b : a ≺ b → a ≼ b.
-  Proof. move=> ab. apply wfo_le_lteq. by left. Qed.
-
-  (** [≼] is transitive *)
-  Lemma wfo_le_trans a b c : a ≼ b → b ≼ c → a ≼ c.
-  Proof.
-    move=> /wfo_le_lteq[ab|<-] /wfo_le_lteq[bc|<-]; apply wfo_le_lteq;
-    [left|by left|by left|by right]. exact (wfo_lt_trans ab bc).
-  Qed.
-
-  (** [≺] is irreflexive *)
-  Lemma wfo_lt_irrefl a : ¬ a ≺ a.
-  Proof.
-    move=> aa. move: (wfo_lt_wf a). fix FIX 1. move=> Acca. apply FIX.
-    apply (Acc_inv Acca aa).
-  Qed.
-End wfo_facts.
+(** [≺] is irreflexive *)
+Lemma wfo_lt_irrefl {A : wfo} (a : A) : ¬ a ≺ a.
+Proof.
+  move=> aa. move: (wfo_lt_wf a). fix FIX 1. move=> Acca. apply FIX.
+  apply (Acc_inv Acca aa).
+Qed.
 
 (** ** Equip [nat] with [lt] *)
 
-Section nat_wfo.
-  Lemma lt_wf : wf lt.
-  Proof. apply well_founded_ltof. Qed.
+Lemma lt_wf : wf lt.
+Proof. apply well_founded_ltof. Qed.
 
-  Canonical nat_wfo := Wfo nat lt le Nat.lt_eq_cases Nat.lt_trans lt_wf.
-End nat_wfo.
+Canonical nat_wfo := Wfo nat lt lt_wf.
